Splinter/Betree/PivotBranch.i.dfy
@@ -7,7 +7,7 @@ include "../../lib/Base/Option.s.dfy"
 include "../../lib/Base/Maps.i.dfy"
 include "../../lib/Base/Sequences.i.dfy"
 include "../../lib/Base/total_order_impl.i.dfy"
-include "Buffers.i.dfy"
+include "Buffer.i.dfy"
 include "Domain.i.dfy"
 
 // Jumping straight to PivotBranch (instead of PagedBranch) since branch is immutable 
@@ -20,7 +20,7 @@ module PivotBranchMod {
   import opened ValueMessage
   import opened Sequences
   import opened DomainMod
-  import opened Buffers
+  import opened BufferMod
   import KeysImpl = Lexicographic_Byte_Order_Impl
   import Keys = KeysImpl.Ord
 
@@ -118,32 +118,17 @@ module PivotBranchMod {
         :: children[Route(key) + 1].I().mapp[key])
     }
 
-    lemma AllKeysIsConsistentWithI(key: Key)
+    function Query(key: Key) : (result: Message)
       requires WF()
-      requires key in I().mapp
-      ensures key in AllKeys()
-      ensures Index? ==> WF() && key in children[Route(key) + 1].AllKeys()
-    {
-    }
-  
-    function Query(key: Key) : (result: Option<Message>)
-      requires WF()
-      ensures result.Some? <==> key in I().mapp
-      ensures result.Some? ==> I().Query(key) == result.value
-      ensures result.None? ==> I().Query(key) == Update(NopDelta())
+      ensures key !in AllKeys() ==> result == Update(NopDelta())
+      ensures result == I().Query(key)
     {
       var r := Route(key);
       if Leaf? then (
         if Route(key) >= 0 && keys[r] == key
-        then Some(msgs[Route(key)]) else None
+        then msgs[Route(key)] else Update(NopDelta())
       ) else (
-        var result := children[Route(key)+1].Query(key);
-        assert result.Some? ==> key in children[Route(key)+1].AllKeys() by {
-          if result.Some? {
-            children[Route(key)+1].AllKeysIsConsistentWithI(key);
-          } 
-        }
-        result
+        children[Route(key)+1].Query(key)
       )
     }
 
@@ -183,59 +168,6 @@ module PivotBranchMod {
       )
     }
 
-    // filter = keys to remove
-    predicate IsFiltered(og: Node, filter: Domain)
-      requires WF()
-      requires og.WF()
-      requires !filter.EmptyDomain?
-    {
-      && (forall k :: Query(k).Some? <==> (!filter.Contains(k) && og.Query(k).Some?))  // define this's domain
-      && (forall k | Query(k).Some? :: Query(k) == og.Query(k)) // value matches og
-    }
-
-    lemma FilteredEquivApplyFilter(og: Node, filter: Domain)
-      requires IsFiltered.requires(og, filter)
-      requires IsFiltered(og, filter)
-      ensures I() == og.I().ApplyFilter(Buffers.AllKeys() - filter.KeySet())
-    {
-      var actual := I();
-      var expected := og.I().ApplyFilter(Buffers.AllKeys() - filter.KeySet());
-
-      assert (forall k :: k in actual.mapp <==> (!filter.Contains(k) && og.Query(k).Some?));
-      assert (forall k :: k in expected.mapp <==> (!filter.Contains(k) && og.Query(k).Some?));
-      assert (forall k :: k in actual.mapp <==> k in expected.mapp);
-
-      assert IsSubMap(actual.mapp, expected.mapp);
-      assert IsSubMap(expected.mapp, actual.mapp);
-      MapEquality(actual.mapp, expected.mapp);
-    }
-  
-    // predicate IsFiltered(og: Node, filter: Domain)
-    //   requires WF()
-    //   requires og.WF()
-    //   requires !filter.EmptyDomain?
-    // {
-    //   && (forall k :: Query(k).Some? <==> (filter.Contains(k) && og.Query(k).Some?))  // define this's domain
-    //   && (forall k | Query(k).Some? :: Query(k) == og.Query(k)) // value matches og
-    // }
-
-    // lemma FilteredEquivApplyFilter(og: Node, filter: Domain)
-    //   requires IsFiltered.requires(og, filter)
-    //   requires IsFiltered(og, filter)
-    //   ensures I() == og.I().ApplyFilter(filter.KeySet())
-    // {
-    //   var actual := I();
-    //   var expected := og.I().ApplyFilter(filter.KeySet());
-
-    //   assert (forall k :: k in actual.mapp <==> (filter.Contains(k) && og.Query(k).Some?));
-    //   assert (forall k :: k in expected.mapp <==> (filter.Contains(k) && og.Query(k).Some?));
-    //   assert (forall k :: k in actual.mapp <==> k in expected.mapp);
-
-    //   assert IsSubMap(actual.mapp, expected.mapp);
-    //   assert IsSubMap(expected.mapp, actual.mapp);
-    //   MapEquality(actual.mapp, expected.mapp);
-    // }
-
     // Note: intended for iterator which we currently don't have
     function Flatten() : (result: FlattenedBranch)
     requires WF()
@@ -256,67 +188,4 @@ module PivotBranchMod {
       && Flatten() == b
     }
   }
-
-  // What can we show if we don't bother with it
-  // we show function is the same as the other function
-  // so as long as we can refine to a valid version of the prior 
-
-  // PivotBranch SM:
-
-  // datatype Variables = Variables(root: Node) {
-  //   predicate WF() {
-  //     && root.WF()
-  //   }
-  // }
-
-  // predicate Query(v: Variables, v': Variables, lbl: TransitionLabel)
-  // {
-  //   && v.WF()
-  //   && lbl.QueryLabel?
-  //   && v.root.Query(lbl.key) == Some(lbl.msg)
-  //   && v' == v
-  // }
-
-  // predicate Filter(v: Variables, v': Variables, lbl: TransitionLabel)
-  // {
-  //   && v.WF()
-  //   && lbl.FilterLabel?
-  //   && lbl.newroot.WF()
-  //   && !lbl.domain.EmptyDomain?
-  //   && lbl.newroot.IsFiltered(v.root, lbl.domain)
-  //   && v'.root == lbl.newroot
-  //   && v'.WF()
-  // }
-
-  // predicate Flatten(v: Variables, v': Variables, lbl: TransitionLabel)
-  // {
-  //   && v.WF()
-  //   && lbl.FlattenLabel?
-  //   && lbl.flattened.WF()
-  //   && v.root.FlattenEquivalent(lbl.flattened)
-  //   && v' == v
-  // }
-
-  // // public: 
-
-  // predicate Init(v: Variables)
-  // {
-  //   && v.WF()
-  // }
-
-  // datatype Step = QueryStep | FilterStep | FlattenStep
-
-  // datatype TransitionLabel =
-  //   QueryLabel(key: Key, msg: Message)
-  // | FilterLabel(newroot: Node, domain: Domain)
-  // | FlattenLabel(flattened: FlattenedBranch)
-
-  // predicate NextStep(v: Variables, v': Variables, lbl: TransitionLabel, step: Step)
-  // {
-  //   match step {
-  //     case QueryStep() => Query(v, v', lbl)
-  //     case FilterStep() => Filter(v, v', lbl)
-  //     case FlattenStep() => Flatten(v, v', lbl)
-  //   }
-  // }
 }
